tests/EraseSimp.lean
@@ -1,0 +1,27 @@
+/-
+Copyright (c) 2023 Jannis Limperg. All rights reserved.
+Released under Apache 2.0 license as described in the file LICENSE.
+Authors: Jannis Limperg
+-/
+
+import Aesop
+
+example (n : Nat) : n + m = m + n := by
+  aesop (add simp Nat.add_comm)
+
+attribute [local simp] Nat.add_comm
+
+example (n : Nat) : n + m = m + n := by
+  aesop
+
+example (n : Nat) : n + m = m + n := by
+  aesop (erase Nat.add_comm) (options := { warnOnNonterminal := false })
+  aesop
+
+example (n : Nat) : n + m = m + n := by
+  aesop (erase norm simp Nat.add_comm) (options := { warnOnNonterminal := false })
+  aesop
+
+example (n : Nat) : n + m = m + n := by
+  aesop (erase apply Nat.add_comm)
+  aesop
